src/fstar/FStarC.CheckedFiles.fsti
@@ -62,7 +62,7 @@ val load_parsing_data_from_cache: file_name:string -> option Parser.Dep.parsing_
 
 //checks if the cache files exists and all their dependences are valid
 //returning the names of all the dependences if so
-val scan_deps_and_check_cache_validity (_:Dep.deps) (file:string) : option (list string & Dep.deps)
+val scan_deps_and_check_cache_validity (file:string) : option (list string & Dep.deps)
 
 val load_module_from_cache: TcEnv.env -> string -> option tc_result
 
